zoo_saturn/bag_2: Verify.

theories/zoo_saturn/bag_2.v
@@ -1,111 +1,629 @@
 From zoo Require Import
   prelude.
+From zoo.common Require Import
+  countable
+  fin_map_dom
+  fin_maps.
+From zoo.iris.bi Require Import
+  big_op.
+From zoo.iris.base_logic Require Import
+  lib.mono_map
+  lib.twins.
 From zoo.language Require Import
   notations.
 From zoo.diaframe Require Import
   diaframe.
 From zoo_std Require Import
-  option.
+  option
+  xtchain.
 From zoo_saturn Require Export
   base
   bag_2__code.
 From zoo_saturn Require Import
-  bag_2__types.
+  bag_2__types
+  spmc_queue.
 From zoo Require Import
   options.
 
+Implicit Types l node 𝑐𝑜𝑛𝑠𝑢𝑚𝑒𝑟 : location.
+Implicit Types nodes : list location.
 Implicit Types v t producer consumer : val.
+Implicit Types o : option val.
+Implicit Types vs ws : list val.
+Implicit Types vss wss : gmap val (list val).
 
 Class Bag2G Σ `{zoo_G : !ZooG Σ} := {
+  #[local] bag_2_G_spmc_queue_G :: SpmcQueueG Σ ;
+  #[local] bag_2_G_queues_G :: MonoMapG Σ location val ;
+  #[local] bag_2_G_model_G :: TwinsG Σ (leibnizO (gmap val (list val))) ;
 }.
 
 Definition bag_2_Σ := #[
+  spmc_queue_Σ ;
+  mono_map_Σ location val ;
+  twins_Σ (leibnizO (gmap val (list val)))
 ].
 #[global] Instance subG_bag_2_Σ Σ `{zoo_G : !ZooG Σ} :
   subG bag_2_Σ Σ →
   Bag2G Σ.
 Proof.
-  (* solve_inG. *)
+  solve_inG.
+Qed.
+
+Record producer := {
+  producer_queue : val ;
+  producer_node : location ;
+}.
+Implicit Types 𝑝𝑟𝑜𝑑𝑢𝑐𝑒𝑟 : producer.
+
+#[local] Coercion producer_to_val 𝑝𝑟𝑜𝑑𝑢𝑐𝑒𝑟 : val :=
+  ( 𝑝𝑟𝑜𝑑𝑢𝑐𝑒𝑟.(producer_queue),
+    #𝑝𝑟𝑜𝑑𝑢𝑐𝑒𝑟.(producer_node)
+  ).
+
+#[local] Lemma producer_eq_alt 𝑝𝑟𝑜𝑑𝑢𝑐𝑒𝑟1 𝑝𝑟𝑜𝑑𝑢𝑐𝑒𝑟2 :
+  𝑝𝑟𝑜𝑑𝑢𝑐𝑒𝑟1.(producer_queue) = 𝑝𝑟𝑜𝑑𝑢𝑐𝑒𝑟2.(producer_queue) →
+  𝑝𝑟𝑜𝑑𝑢𝑐𝑒𝑟1.(producer_node) = 𝑝𝑟𝑜𝑑𝑢𝑐𝑒𝑟2.(producer_node) →
+  𝑝𝑟𝑜𝑑𝑢𝑐𝑒𝑟1 = 𝑝𝑟𝑜𝑑𝑢𝑐𝑒𝑟2.
+Proof.
+  destruct 𝑝𝑟𝑜𝑑𝑢𝑐𝑒𝑟1, 𝑝𝑟𝑜𝑑𝑢𝑐𝑒𝑟2; naive_solver.
+Qed.
+#[local] Instance producer_to_val_inj :
+  Inj (=) (=) producer_to_val.
+Proof.
+  intros [] []; naive_solver.
+Qed.
+
+Record descriptor := {
+  descriptor_queue : val ;
+  descriptor_vals : list val ;
+}.
+Implicit Types descr : descriptor.
+Implicit Types descrs : gmap location descriptor.
+
+#[local] Definition descriptor_update_vals descr f :=
+  {|descriptor_queue := descr.(descriptor_queue) ;
+    descriptor_vals := f descr.(descriptor_vals) ;
+  |}.
+
+#[local] Definition descriptor_to_producer descr node :=
+  {|producer_queue := descr.(descriptor_queue) ;
+    producer_node := node ;
+  |}.
+
+#[local] Lemma descriptor_to_producer_inj descr1 node1 descr2 node2 :
+  descriptor_to_producer descr1 node1 = descriptor_to_producer descr2 node2 →
+  node1 = node2.
+Proof.
+  naive_solver.
 Qed.
 
 Section bag_2_G.
   Context `{bag_2_G : Bag2G Σ}.
 
-  Parameter bag_2_inv : val → namespace → iProp Σ.
+  Record metadata := {
+    metadata_inv : namespace ;
+    metadata_model : gname ;
+    metadata_queues : gname ;
+  }.
+  Implicit Types γ : metadata.
 
-  Parameter bag_2_model : val → list (list val) → iProp Σ.
-
-  Parameter bag_2_producer : val → val → nat → list val → iProp Σ.
-
-  Parameter bag_2_consumer : val → val → iProp Σ.
-
-  #[global] Instance bag_2_model_timeless t vs :
-    Timeless (bag_2_model t vs).
+  #[local] Instance metadata_eq_dec : EqDecision metadata :=
+    ltac:(solve_decision).
+  #[local] Instance metadata_countable :
+    Countable metadata.
   Proof.
-  Admitted.
-  #[global] Instance bag_2_producer_timeless t producer i ws :
-    Timeless (bag_2_producer t producer i ws).
+    solve_countable.
+  Qed.
+
+  #[local] Definition queues_auth' γ_queues nodes descrs wss : iProp Σ :=
+    mono_map_auth γ_queues (DfracOwn 1) (descriptor_queue <$> descrs) ∗
+    ⌜dom descrs = list_to_set nodes⌝ ∗
+    ⌜ map_Forall (λ node descr,
+        wss !! (descriptor_to_producer descr node : val) = Some descr.(descriptor_vals)
+      ) descrs
+    ⌝.
+  #[local] Instance : CustomIpatFormat "queues_auth" :=
+    "(
+      Hauth &
+      %Hnodes &
+      %Hdescrs
+    )".
+  #[local] Definition queues_auth γ :=
+    queues_auth' γ.(metadata_queues).
+  #[local] Definition queues_at' :=
+    mono_map_at.
+  #[local] Definition queues_at γ :=
+    queues_at' γ.(metadata_queues).
+  #[local] Definition queues_elem γ queue : iProp Σ :=
+    match queue with
+    | None =>
+        True
+    | Some queue =>
+        ∃ node,
+        queues_at γ node queue ∗
+        spmc_queue_inv queue (γ.(metadata_inv).@"producer")
+    end.
+  #[local] Instance : CustomIpatFormat "queues_elem" :=
+    "(
+      %node &
+      #Hqueues_at &
+      #Hqueue_inv
+    )".
+
+  #[local] Definition model₁' γ_model vss :=
+    twins_twin1 γ_model (DfracOwn 1) vss.
+  #[local] Definition model₁ γ :=
+    model₁' γ.(metadata_model).
+  #[local] Definition model₂' γ_model vss :=
+    twins_twin2 γ_model vss.
+  #[local] Definition model₂ γ :=
+    model₂' γ.(metadata_model).
+
+  #[local] Definition descriptor_model γ node descr : iProp Σ :=
+    ∃ o,
+    node.[queue] ↦ o ∗
+    ⌜from_option (.= descr.(descriptor_queue)) True o⌝ ∗
+    spmc_queue_inv descr.(descriptor_queue) (γ.(metadata_inv).@"producer") ∗
+    spmc_queue_model descr.(descriptor_queue) descr.(descriptor_vals).
+  #[local] Instance : CustomIpatFormat "descriptor_model" :=
+    "(
+      %o{} &
+      Hnode{}_queue &
+      {>=}%Ho{} &
+      {{inv}#Hqueue{}_inv={inv}#Hqueue_inv=_} &
+      {>=}Hqueue{}_model
+    )".
+
+  #[local] Definition inv_inner l γ : iProp Σ :=
+    ∃ nodes descrs wss,
+    l.[producers] ↦ from_option #@{location} §Null (head nodes) ∗
+    xtchain (Header §Node 2) DfracDiscarded nodes §Null ∗
+    queues_auth γ nodes descrs wss ∗
+    model₂ γ wss ∗
+    [∗ map] node ↦ descr ∈ descrs,
+      descriptor_model γ node descr.
+  #[local] Instance : CustomIpatFormat "inv_inner" :=
+    "(
+      %nodes{} &
+      %descrs{} &
+      %wss &
+      Hl_producers &
+      Hnodes{} &
+      >Hqueues_auth &
+      >Hmodel₂ &
+      Hdescrs
+    )".
+  #[local] Definition inv' l γ :=
+    inv (γ.(metadata_inv).@"inv") (inv_inner l γ).
+  Definition bag_2_inv t ι : iProp Σ :=
+    ∃ l γ,
+    ⌜t = #l⌝ ∗
+    ⌜ι = γ.(metadata_inv)⌝ ∗
+    meta l nroot γ ∗
+    inv' l γ.
+  #[local] Instance : CustomIpatFormat "inv" :=
+    "(
+      %l &
+      %γ &
+      -> &
+      -> &
+      #Hmeta &
+      #Hinv
+    )".
+
+  Definition bag_2_model t vss : iProp Σ :=
+    ∃ l γ,
+    ⌜t = #l⌝ ∗
+    meta l nroot γ ∗
+    model₁ γ vss.
+  #[local] Instance : CustomIpatFormat "model" :=
+    "(
+      %l{=_} &
+      %γ{=_} &
+      %Heq{} &
+      #Hmeta_{} &
+      Hmodel₁
+    )".
+
+  Definition bag_2_producer t producer ws : iProp Σ :=
+    ∃ l γ 𝑝𝑟𝑜𝑑𝑢𝑐𝑒𝑟,
+    ⌜t = #l⌝ ∗
+    ⌜producer = 𝑝𝑟𝑜𝑑𝑢𝑐𝑒𝑟⌝ ∗
+    meta l nroot γ ∗
+    𝑝𝑟𝑜𝑑𝑢𝑐𝑒𝑟.(producer_node) ↦ₕ Header §Node 2 ∗
+    queues_at γ 𝑝𝑟𝑜𝑑𝑢𝑐𝑒𝑟.(producer_node) 𝑝𝑟𝑜𝑑𝑢𝑐𝑒𝑟.(producer_queue) ∗
+    spmc_queue_inv 𝑝𝑟𝑜𝑑𝑢𝑐𝑒𝑟.(producer_queue) (γ.(metadata_inv).@"producer") ∗
+    spmc_queue_producer 𝑝𝑟𝑜𝑑𝑢𝑐𝑒𝑟.(producer_queue) ws.
+  #[local] Instance : CustomIpatFormat "producer" :=
+    "(
+      %l{=_} &
+      %γ{=_} &
+      %𝑝𝑟𝑜𝑑𝑢𝑐𝑒𝑟{} &
+      %Ht_eq{} &
+      {%Hproducer_eq{}=->} &
+      #Hmeta{_{}=_} &
+      #Hnode_header{_{}} &
+      #Hqueues_at{_{}} &
+      #Hqueue_inv{_{}} &
+      Hqueue_producer{_{}}
+    )".
+
+  Definition bag_2_consumer t consumer : iProp Σ :=
+    ∃ l γ 𝑐𝑜𝑛𝑠𝑢𝑚𝑒𝑟 (queue : option val),
+    ⌜t = #l⌝ ∗
+    meta l nroot γ ∗
+    ⌜consumer = #𝑐𝑜𝑛𝑠𝑢𝑚𝑒𝑟⌝ ∗
+    𝑐𝑜𝑛𝑠𝑢𝑚𝑒𝑟.[consumer_queue] ↦ queue ∗
+    queues_elem γ queue.
+  #[local] Instance : CustomIpatFormat "consumer" :=
+    "(
+      %l_ &
+      %γ_ &
+      %𝑐𝑜𝑛𝑠𝑢𝑚𝑒𝑟 &
+      %queue &
+      %Heq &
+      Hmeta_ &
+      -> &
+      Hconsumer_queue &
+      #Hqueues_elem
+    )".
+
+  #[local] Instance queues_auth_timeless γ nodes descrs wss :
+    Timeless (queues_auth γ nodes descrs wss).
   Proof.
-  Admitted.
-  #[global] Instance bag_2_consumer_timeless t consumer :
-    Timeless (bag_2_consumer t consumer).
+    apply _.
+  Qed.
+  #[global] Instance bag_2_model_timeless t vss :
+    Timeless (bag_2_model t vss).
   Proof.
-  Admitted.
+    apply _.
+  Qed.
   #[global] Instance bag_2_inv_persistent t ι :
     Persistent (bag_2_inv t ι).
   Proof.
-  Admitted.
+    apply _.
+  Qed.
 
-  Lemma bag_2_producer_valid t vss producer i ws :
+  #[local] Lemma queues_alloc :
+    ⊢ |==>
+      ∃ γ_queues,
+      queues_auth' γ_queues [] ∅ ∅.
+  Proof.
+    iMod mono_map_alloc as "(%γ_queues & Hauth)".
+    iSteps.
+  Qed.
+  #[local] Lemma queues_at_get {γ nodes descrs wss} i node :
+    nodes !! i = Some node →
+    queues_auth γ nodes descrs wss ⊢
+      ∃ descr,
+      ⌜descrs !! node = Some descr⌝ ∗
+      queues_at γ node descr.(descriptor_queue).
+  Proof.
+    iIntros "%Hnodes_lookup (:queues_auth)".
+    destruct (elem_of_dom_1 descrs node) as (descr & Hdescrs_lookup).
+    { rewrite Hnodes elem_of_list_to_set elem_of_list_lookup. eauto. }
+    iDestruct (mono_map_at_get with "Hauth") as "#Hat".
+    { rewrite lookup_fmap_Some. eauto. }
+    iSteps.
+  Qed.
+  #[local] Lemma queues_at_valid γ nodes descrs wss node queue :
+    queues_auth γ nodes descrs wss -∗
+    queues_at γ node queue -∗
+      ∃ descr,
+      ⌜descrs !! node = Some descr⌝ ∗
+      ⌜descr.(descriptor_queue) = queue⌝ ∗
+      ⌜wss !! (descriptor_to_producer descr node : val) = Some descr.(descriptor_vals)⌝.
+  Proof.
+    iIntros "(:queues_auth) Hat".
+    iDestruct (mono_map_at_valid with "Hauth Hat") as %(descr & ? & Hdescrs_lookup)%lookup_fmap_Some.
+    iSteps.
+  Qed.
+  #[local] Lemma queues_at_valid_producer γ nodes descrs wss 𝑝𝑟𝑜𝑑𝑢𝑐𝑒𝑟 :
+    queues_auth γ nodes descrs wss -∗
+    queues_at γ 𝑝𝑟𝑜𝑑𝑢𝑐𝑒𝑟.(producer_node) 𝑝𝑟𝑜𝑑𝑢𝑐𝑒𝑟.(producer_queue) -∗
+      ∃ descr,
+      ⌜descrs !! 𝑝𝑟𝑜𝑑𝑢𝑐𝑒𝑟.(producer_node) = Some descr⌝ ∗
+      ⌜descr.(descriptor_queue) = 𝑝𝑟𝑜𝑑𝑢𝑐𝑒𝑟.(producer_queue)⌝ ∗
+      ⌜wss !! (𝑝𝑟𝑜𝑑𝑢𝑐𝑒𝑟 : val) = Some descr.(descriptor_vals)⌝.
+  Proof.
+    iIntros "Hauth Hat".
+    iDestruct (queues_at_valid with "Hauth Hat") as "(%descr & %Hdescrs_lookup & %Hdescr_queue & %Hwss_lookup)".
+    rewrite (producer_eq_alt 𝑝𝑟𝑜𝑑𝑢𝑐𝑒𝑟 (descriptor_to_producer descr 𝑝𝑟𝑜𝑑𝑢𝑐𝑒𝑟.(producer_node))) //.
+    iSteps.
+  Qed.
+  #[local] Lemma queues_insert {γ nodes descrs wss} node descr :
+    descrs !! node = None →
+    queues_auth γ nodes descrs wss ⊢ |==>
+      queues_auth γ
+        (node :: nodes)
+        (<[node := descr]> descrs)
+        (<[descriptor_to_producer descr node : val := descr.(descriptor_vals)]> wss) ∗
+      queues_at γ node descr.(descriptor_queue).
+  Proof.
+    iIntros "%Hdescrs_lookup (:queues_auth)".
+    iMod (mono_map_insert' node descr.(descriptor_queue) with "Hauth") as "(Hauth & Hat)".
+    { rewrite lookup_fmap Hdescrs_lookup //. }
+    rewrite -fmap_insert. iSteps; iPureIntro.
+    - set_solver.
+    - apply map_Forall_insert_2.
+      + rewrite lookup_insert //.
+      + eapply map_Forall_impl'; first done. move=> /= node' descr' Hdescrs_lookup' Hwss_lookup.
+        destruct (decide (node' = node)) as [-> |].
+        * simplify.
+        * rewrite lookup_insert_ne //.
+          intros ?%(inj _)%descriptor_to_producer_inj. done.
+  Qed.
+  #[local] Lemma queues_update {γ nodes descrs wss} node descr f :
+    descrs !! node = Some descr →
+    queues_auth γ nodes descrs wss ⊢
+    queues_auth γ
+      nodes
+      (<[node := descriptor_update_vals descr f]> descrs)
+      (<[descriptor_to_producer descr node : val := f descr.(descriptor_vals)]> wss).
+  Proof.
+    iIntros "%Hdescrs_lookup (:queues_auth)".
+    rewrite /queues_auth /queues_auth'.
+    rewrite fmap_insert /= -fmap_insert insert_id //.
+    iFrame. iSplit; iPureIntro.
+    - rewrite dom_insert_lookup_L //.
+    - apply map_Forall_insert_2'.
+      + rewrite lookup_insert //.
+      + apply map_Forall_delete_lookup => node' descr' Hnode' Hdescrs_lookup'.
+        rewrite lookup_insert_ne; first naive_solver.
+        rewrite map_Forall_lookup in Hdescrs. auto.
+  Qed.
+  #[local] Lemma queues_update_producer {γ nodes descrs wss} 𝑝𝑟𝑜𝑑𝑢𝑐𝑒𝑟 descr f :
+    descrs !! 𝑝𝑟𝑜𝑑𝑢𝑐𝑒𝑟.(producer_node) = Some descr →
+    descr.(descriptor_queue) = 𝑝𝑟𝑜𝑑𝑢𝑐𝑒𝑟.(producer_queue) →
+    queues_auth γ nodes descrs wss ⊢
+    queues_auth γ
+      nodes
+      (<[𝑝𝑟𝑜𝑑𝑢𝑐𝑒𝑟.(producer_node) := descriptor_update_vals descr f]> descrs)
+      (<[𝑝𝑟𝑜𝑑𝑢𝑐𝑒𝑟 : val := f descr.(descriptor_vals)]> wss).
+  Proof.
+    intros Hdescrs_lookup Hdescr_queue.
+    rewrite (queues_update 𝑝𝑟𝑜𝑑𝑢𝑐𝑒𝑟.(producer_node) descr f) //.
+    rewrite /descriptor_to_producer Hdescr_queue //.
+  Qed.
+
+  #[local] Lemma model_alloc :
+    ⊢ |==>
+      ∃ γ_model,
+      model₁' γ_model ∅ ∗
+      model₂' γ_model ∅.
+  Proof.
+    apply twins_alloc'.
+  Qed.
+  #[local] Lemma model_agree γ vss1 vss2 :
+    model₁ γ vss1 -∗
+    model₂ γ vss2 -∗
+    ⌜vss1 = vss2⌝.
+  Proof.
+    apply: twins_agree_L.
+  Qed.
+  #[local] Lemma model_update {γ vss1 vss2} vss :
+    model₁ γ vss1 -∗
+    model₂ γ vss2 ==∗
+      model₁ γ vss ∗
+      model₂ γ vss.
+  Proof.
+    apply twins_update'.
+  Qed.
+
+  Opaque queues_auth'.
+
+  Lemma bag_2_producer_valid t ι vss producer ws E :
+    ↑ι ⊆ E →
+    bag_2_inv t ι -∗
     bag_2_model t vss -∗
-    bag_2_producer t producer i ws -∗
+    bag_2_producer t producer ws ={E}=∗
       ∃ vs,
-      ⌜vss !! i = Some vs⌝ ∗
+      ⌜vss !! producer = Some vs⌝ ∗
       ⌜vs `suffix_of` ws⌝.
   Proof.
-  Admitted.
+    iIntros "% (:inv) (:model =1) (:producer =2)". simplify.
+    iDestruct (meta_agree with "Hmeta Hmeta_1") as %<-. iClear "Hmeta_1".
+    iDestruct (meta_agree with "Hmeta Hmeta_2") as %<-. iClear "Hmeta_2".
+
+    iInv "Hinv" as "(:inv_inner)".
+    iDestruct (model_agree with "Hmodel₁ Hmodel₂") as %<-.
+    iDestruct (queues_at_valid_producer with "Hqueues_auth Hqueues_at_2") as %(descr & Hdescrs_lookup & Hdescr_queue & Hvss_lookup).
+    iAssert (◇ ⌜descr.(descriptor_vals) `suffix_of` ws⌝)%I as "#>%".
+    { iDestruct (big_sepM_lookup with "Hdescrs") as "(:descriptor_model >)"; first done.
+      rewrite Hdescr_queue.
+      iApply (spmc_queue_producer_valid with "Hqueue_producer_2 Hqueue_model").
+    }
+    iSplitL. { iFrameSteps. }
+    iSteps.
+  Qed.
+  Lemma bag_2_producer_exclusive t producer ws1 ws2 :
+    bag_2_producer t producer ws1 -∗
+    bag_2_producer t producer ws2 -∗
+    False.
+  Proof.
+    iIntros "(:producer =1) (:producer =2)". simplify.
+    iApply (spmc_queue_producer_exclusive with "Hqueue_producer_1 Hqueue_producer_2").
+  Qed.
 
   Lemma bag_2_create_spec ι :
     {{{
       True
     }}}
-      bag_2_create  ()
+      bag_2_create ()
     {{{ t,
       RET t;
       bag_2_inv t ι ∗
-      bag_2_model t []
+      bag_2_model t ∅
     }}}.
   Proof.
-  Admitted.
+    iIntros "%Φ _ HΦ".
 
+    wp_rec.
+    wp_block l as "Hmeta" "(Hl_producers & _)".
+
+    iMod model_alloc as "(%γ_model & Hmodel₁ & Hmodel₂)".
+    iMod queues_alloc as "(%γ_queues & Hqueues_auth)".
+
+    pose γ := {|
+      metadata_inv := ι ;
+      metadata_model := γ_model ;
+      metadata_queues := γ_queues ;
+    |}.
+    iMod (meta_set γ with "Hmeta") as "#Hmeta"; first done.
+
+    iApply "HΦ".
+    iSplitR "Hmodel₁"; last iSteps.
+    iExists l, γ. iStep 3. iApply inv_alloc. iFrame.
+    iDestruct xtchain_nil as "$".
+    rewrite big_sepM_empty. iSteps.
+  Qed.
+
+  #[local] Lemma bag_2_add_producer_0_spec l γ (queue : val) :
+    <<<
+      meta l nroot γ ∗
+      inv' l γ ∗
+      spmc_queue_inv queue (γ.(metadata_inv).@"producer") ∗
+      spmc_queue_model queue []
+    | ∀∀ vss,
+      model₁ γ vss
+    >>>
+      bag_2_add_producer_0 #l (Some queue) @ ↑γ.(metadata_inv)
+    <<<
+      ∃∃ node,
+      let 𝑝𝑟𝑜𝑑𝑢𝑐𝑒𝑟 := {|
+        producer_queue := queue ;
+        producer_node := node ;
+      |} in
+      model₁ γ (<[𝑝𝑟𝑜𝑑𝑢𝑐𝑒𝑟 : val := []]> vss)
+    | RET #node;
+      node ↦ₕ Header §Node 2 ∗
+      queues_at γ node queue
+    >>>.
+  Proof.
+    iIntros "%Φ (#Hmeta & #Hinv & #Hqueue_inv & Hqueue_model) HΦ".
+    iLöb as "HLöb".
+
+    wp_rec. wp_pures.
+
+    wp_bind (_.{producers})%E.
+    iInv "Hinv" as "(:inv_inner =1)".
+    wp_load.
+    iSplitR "Hqueue_model HΦ". { iFrameSteps. }
+    iIntros "!> {%}".
+
+    wp_block node as "#Hnode_header" "_" "(Hnode_next & Hnode_queue & _)".
+    iMod (pointsto_persist with "Hnode_next") as "#Hnode_next".
+    wp_match. wp_pures.
+
+    wp_bind (CAS _ _ _).
+    iInv "Hinv" as "(:inv_inner =2)".
+    wp_cas as Hcas; first iSteps.
+    assert (head nodes1 = head nodes2) as ->.
+    { destruct nodes1, nodes2; zoo_simpl; done. }
+    iDestruct (xtchain_cons_2 with "Hnode_header [] Hnodes2") as "Hnodes"; first iSteps.
+
+    iAssert ⌜descrs2 !! node = None⌝%I as %Hdescr2_lookup.
+    { rewrite eq_None_not_Some. iIntros "(%descr' & %)".
+      iDestruct (big_sepM_lookup with "Hdescrs") as "(:descriptor_model =')"; first done.
+      iApply (pointsto_exclusive with "Hnode_queue Hnode'_queue").
+    }
+
+    pose descr := {|
+      descriptor_queue := queue ;
+      descriptor_vals := [] ;
+    |}.
+    iMod (queues_insert node descr with "Hqueues_auth") as "(Hqueues_auth & #Hqueues_at)"; first done.
+    iDestruct (big_sepM_insert_2 _ _ node descr with "[Hnode_queue Hqueue_model] Hdescrs") as "Hdescrs".
+    { iExists (Some queue). iSteps. }
+
+    iMod "HΦ" as "(%vss & Hmodel₁ & _ & HΦ)".
+    iDestruct (model_agree with "Hmodel₁ Hmodel₂") as %<-.
+    set vss' :=
+      <[descriptor_to_producer descr node : val := []]> vss.
+    iMod (model_update vss' with "Hmodel₁ Hmodel₂") as "(Hmodel₁ & Hmodel₂)".
+    iMod ("HΦ" with "Hmodel₁ [$Hnode_header $Hqueues_at]") as "HΦ".
+
+    iSplitR "HΦ". { iFrameSteps. }
+    iSteps.
+  Qed.
+  #[local] Lemma bag_2_add_producer_spec l γ (queue : val) :
+    <<<
+      meta l nroot γ ∗
+      inv' l γ ∗
+      spmc_queue_inv queue (γ.(metadata_inv).@"producer") ∗
+      spmc_queue_model queue []
+    | ∀∀ vss,
+      model₁ γ vss
+    >>>
+      bag_2_add_producer #l queue @ ↑γ.(metadata_inv)
+    <<<
+      ∃∃ node,
+      let 𝑝𝑟𝑜𝑑𝑢𝑐𝑒𝑟 := {|
+        producer_queue := queue ;
+        producer_node := node ;
+      |} in
+      model₁ γ (<[𝑝𝑟𝑜𝑑𝑢𝑐𝑒𝑟 : val := []]> vss)
+    | RET #node;
+      node ↦ₕ Header §Node 2 ∗
+      queues_at γ node queue
+    >>>.
+  Proof.
+    iIntros "%Φ H HΦ".
+
+    wp_rec.
+    wp_smart_apply (bag_2_add_producer_0_spec with "H HΦ").
+  Qed.
   Lemma bag_2_create_producer_spec t ι :
     <<<
       bag_2_inv t ι
     | ∀∀ vss,
       bag_2_model t vss
     >>>
-      bag_2_create_producer t
+      bag_2_create_producer t @ ↑ι
     <<<
-      bag_2_model t (vss ++ [[]])
-    | prod,
-      RET prod;
-      bag_2_producer t prod (length vss) []
+      ∃∃ producer,
+      bag_2_model t (<[producer := []]> vss)
+    | RET producer;
+      bag_2_producer t producer []
     >>>.
   Proof.
-  Admitted.
+    iIntros "%Φ (:inv) HΦ".
 
-  Lemma bag_2_close_producer_spec t ι producer i ws :
+    wp_rec.
+    wp_apply (spmc_queue_create_spec with "[//]") as (queue) "(#Hqueue_inv & Hqueue_model & Hqueue_producer)".
+
+    awp_smart_apply (bag_2_add_producer_spec with "[$Hmeta $Hinv $Hqueue_inv $Hqueue_model]") without "Hqueue_producer".
+    iApply (aacc_aupd_commit with "HΦ"); first done. iIntros "%vss (:model)". injection Heq as <-.
+    iDestruct (meta_agree with "Hmeta Hmeta_") as %<-. iClear "Hmeta_".
+    iAaccIntro with "Hmodel₁"; iSteps.
+  Qed.
+
+  Lemma bag_2_close_producer_spec t ι producer ws :
     {{{
       bag_2_inv t ι ∗
-      bag_2_producer t producer i ws
+      bag_2_producer t producer ws
     }}}
       bag_2_close_producer producer
     {{{
       RET ();
-      bag_2_producer t producer i ws
+      bag_2_producer t producer ws
     }}}.
   Proof.
-  Admitted.
+    iIntros "%Φ ((:inv) & (:producer)) HΦ". injection Ht_eq as <-.
+    iDestruct (meta_agree with "Hmeta Hmeta_") as %<-. iClear "Hmeta_".
+
+    wp_rec. wp_match.
+
+    iInv "Hinv" as "(:inv_inner)".
+    iDestruct (queues_at_valid_producer with "Hqueues_auth Hqueues_at") as %(descr & Hdescrs_lookup & Hdescr_queue & Hwss_lookup).
+    iDestruct (big_sepM_lookup_acc with "Hdescrs") as "((:descriptor_model >) & Hdescrs)"; first done.
+    wp_store.
+    iDestruct ("Hdescrs" with "[Hnode_queue Hqueue_model]") as "Hdescrs".
+    { iExists None. rewrite Hdescr_queue. iSteps. }
+    iSplitR "Hqueue_producer HΦ". { iFrameSteps. }
+    iSteps.
+  Qed.
 
   Lemma bag_2_create_consumer_spec t ι :
     {{{
@@ -117,26 +635,210 @@ Section bag_2_G.
       bag_2_consumer t consumer
     }}}.
   Proof.
-  Admitted.
+    iIntros "%Φ (:inv) HΦ".
 
-  Lemma bag_2_push_spec t ι producer i ws v :
+    wp_rec.
+    wp_block 𝑐𝑜𝑛𝑠𝑢𝑚𝑒𝑟 as "(Hconsumer_queue & _)".
+    iSteps. iExists None. iSteps.
+  Qed.
+
+  Lemma bag_2_push_spec t ι producer ws v :
     <<<
       bag_2_inv t ι ∗
-      bag_2_producer t producer i ws
+      bag_2_producer t producer ws
     | ∀∀ vss,
       bag_2_model t vss
     >>>
-      bag_2_push producer v
+      bag_2_push producer v @ ↑ι
     <<<
       ∃∃ vs,
-      ⌜vss !! i = Some vs⌝ ∗
-      bag_2_model t (<[i := vs ++ [v]]> vss)
+      ⌜vss !! producer = Some vs⌝ ∗
+      bag_2_model t (<[producer := vs ++ [v]]> vss)
     | RET ();
-      bag_2_producer t producer i (ws ++ [v])
+      bag_2_producer t producer (vs ++ [v])
     >>>.
   Proof.
-  Admitted.
+    iIntros "%Φ ((:inv) & (:producer)) HΦ". injection Ht_eq as <-.
+    iDestruct (meta_agree with "Hmeta Hmeta_") as %<-. iClear "Hmeta_".
 
+    wp_rec.
+
+    awp_smart_apply (spmc_queue_push_spec with "[$Hqueue_inv $Hqueue_producer]").
+    iInv "Hinv" as "(:inv_inner)".
+    iDestruct (queues_at_valid_producer with "Hqueues_auth Hqueues_at") as %(descr & Hdescrs_lookup & Hdescr_queue & Hwss_lookup). rewrite -Hdescr_queue.
+    iDestruct (big_sepM_insert_acc with "Hdescrs") as "((:descriptor_model >) & Hdescrs)"; first done.
+    iAaccIntro with "Hqueue_model"; iIntros "Hqueue_model".
+    { iDestruct ("Hdescrs" with "[Hnode_queue Hqueue_model]") as "Hdescrs"; first iSteps.
+      rewrite insert_id //. iFrameSteps.
+    }
+    iDestruct (queues_update_producer 𝑝𝑟𝑜𝑑𝑢𝑐𝑒𝑟 descr (.++ [v]) with "Hqueues_auth") as "Hqueues_auth"; [done.. |].
+    set descr' :=
+      descriptor_update_vals descr (.++ [v]).
+    iDestruct ("Hdescrs" $! descr' with "[Hnode_queue Hqueue_model]") as "Hdescrs"; first iSteps.
+
+    iMod "HΦ" as "(%vss & (:model) & _ & HΦ)". injection Heq as <-.
+    iDestruct (meta_agree with "Hmeta Hmeta_") as %<-. iClear "Hmeta_".
+    iDestruct (model_agree with "Hmodel₁ Hmodel₂") as %<-.
+    set vss' :=
+      <[𝑝𝑟𝑜𝑑𝑢𝑐𝑒𝑟 : val := descr.(descriptor_vals) ++ [v]]> vss.
+    iMod (model_update vss' with "Hmodel₁ Hmodel₂") as "(Hmodel₁ & Hmodel₂)".
+    iMod ("HΦ" with "[Hmodel₁]") as "HΦ"; first iSteps.
+
+    iSplitR "HΦ". { iFrameSteps. }
+    rewrite Hdescr_queue. iSteps.
+  Qed.
+
+  #[local] Lemma bag_2_pop_0_spec l γ 𝑐𝑜𝑛𝑠𝑢𝑚𝑒𝑟 (queue : option val) nodes :
+    <<<
+      meta l nroot γ ∗
+      inv' l γ ∗
+      𝑐𝑜𝑛𝑠𝑢𝑚𝑒𝑟.[consumer_queue] ↦ queue ∗
+      queues_elem γ queue ∗
+      xtchain (Header §Node 2) DfracDiscarded nodes §Null ∗
+      [∗ list] node ∈ nodes,
+        ∃ queue,
+        queues_at γ node queue
+    | ∀∀ vss,
+      model₁ γ vss
+    >>>
+      bag_2_pop_0 #𝑐𝑜𝑛𝑠𝑢𝑚𝑒𝑟 (from_option #@{location} §Null%V $ head nodes) @ ↑γ.(metadata_inv)
+    <<<
+      ∃∃ o,
+      match o with
+      | None =>
+          model₁ γ vss
+      | Some v =>
+          ∃ producer vs,
+          ⌜vss !! producer = Some (v :: vs)⌝ ∗
+          model₁ γ (<[producer := vs]> vss)
+      end
+    | queue : option val,
+      RET o;
+      𝑐𝑜𝑛𝑠𝑢𝑚𝑒𝑟.[consumer_queue] ↦ queue ∗
+      queues_elem γ queue
+    >>>.
+  Proof.
+    iIntros "%Φ (#Hmeta & #Hinv & Hconsumer_queue & #Hqueues_elem & Hnodes & Hqueues_ats) HΦ".
+
+    iLöb as "HLöb" forall (nodes).
+
+    wp_rec.
+    destruct nodes as [| node nodes].
+
+    - wp_pures.
+
+      iMod "HΦ" as "(%vss & Hmodel₁ & _ & HΦ)".
+      iMod ("HΦ" $! None with "Hmodel₁") as "HΦ".
+
+      iSteps.
+
+    - iDestruct (xtchain_cons' with "Hnodes") as "-#(#Hnode_header & #Hnode_next & #Hnodes)".
+      iDestruct (big_sepL_cons_1 with "Hqueues_ats") as "-#((%queue0 & #Hqueues_at) & #Hqueues_ats)".
+      wp_match.
+
+      wp_bind (_.{queue})%E.
+      iInv "Hinv" as "(:inv_inner =1)".
+      iDestruct (queues_at_valid with "Hqueues_auth Hqueues_at") as "#(%descr & %Hdescrs1_lookup & %Hdescr_queue & _)".
+      iDestruct (big_sepM_lookup_acc with "Hdescrs") as "((:descriptor_model =0 > inv=) & Hdescrs)"; first done.
+      wp_load.
+      iSplitR "Hconsumer_queue HΦ". { iFrameSteps. }
+      rewrite Hdescr_queue. iIntros "!>".
+
+      destruct o0 as [queue0_ |]; wp_pures.
+
+      + rewrite Ho0 Hdescr_queue. clear.
+
+        awp_smart_apply (spmc_queue_pop_spec with "Hqueue0_inv") without "Hconsumer_queue".
+        iInv "Hinv" as "(:inv_inner =2)".
+        iDestruct (queues_at_valid with "Hqueues_auth Hqueues_at") as "(%descr & %Hdescrs_lookup & %Hdescr_queue & %Hwss_lookup)".
+        iDestruct (big_sepM_insert_acc with "Hdescrs") as "((:descriptor_model >) & Hdescrs)"; first done.
+        rewrite -Hdescr_queue.
+        iAaccIntro with "Hqueue_model"; iIntros "Hqueue_model".
+        { iDestruct ("Hdescrs" with "[Hnode_queue Hqueue_model]") as "Hdescrs"; first iSteps.
+          rewrite insert_id //. iFrameSteps.
+        }
+        destruct descr.(descriptor_vals) as [| v vs] eqn:Hdescr_vals => /=.
+
+        * iDestruct ("Hdescrs" with "[Hnode_queue Hqueue_model]") as "Hdescrs".
+          { rewrite -Hdescr_vals. iFrameSteps. }
+          rewrite insert_id //.
+          iSplitR "HΦ". { iFrameSteps. }
+          iIntros "{%} !> _ Hconsumer_queue".
+
+          wp_load.
+          wp_apply ("HLöb" $! nodes with "Hconsumer_queue Hnodes [$] HΦ").
+
+        * iMod "HΦ" as "(%vss & Hmodel₁ & _ & HΦ)".
+          iDestruct (model_agree with "Hmodel₁ Hmodel₂") as %<-.
+          set vss' :=
+            <[descriptor_to_producer descr node : val := vs]> vss.
+          iMod (model_update vss' with "Hmodel₁ Hmodel₂") as "(Hmodel₁ & Hmodel₂)".
+          iMod ("HΦ" $! (Some v) with "[Hmodel₁]") as "HΦ"; first iSteps.
+
+          iDestruct (queues_update node descr (const vs) with "Hqueues_auth") as "Hqueues_auth"; first done.
+          set descr' :=
+            descriptor_update_vals descr (const vs).
+          iDestruct ("Hdescrs" $! descr' with "[Hnode_queue Hqueue_model]") as "Hdescrs"; first iFrameSteps.
+
+          iSplitR "HΦ". { iFrameSteps. }
+          iSteps. iExists (Some _). iSteps.
+
+      + wp_load.
+        wp_apply ("HLöb" $! nodes with "Hconsumer_queue Hnodes [$] HΦ").
+  Qed.
+  #[local] Lemma bag_2_pop_1_spec t ι consumer :
+    <<<
+      bag_2_inv t ι ∗
+      bag_2_consumer t consumer
+    | ∀∀ vss,
+      bag_2_model t vss
+    >>>
+      bag_2_pop_1 t consumer @ ↑ι
+    <<<
+      ∃∃ o,
+      match o with
+      | None =>
+          bag_2_model t vss
+      | Some v =>
+          ∃ producer vs,
+          ⌜vss !! producer = Some (v :: vs)⌝ ∗
+          bag_2_model t (<[producer := vs]> vss)
+      end
+    | RET o;
+      bag_2_consumer t consumer
+    >>>.
+  Proof.
+    iIntros "%Φ ((:inv) & (:consumer)) HΦ". injection Heq as <-.
+    iDestruct (meta_agree with "Hmeta Hmeta_") as %<-. iClear "Hmeta_".
+
+    wp_rec. wp_pures.
+
+    wp_bind (_.{producers})%E.
+    iInv "Hinv" as "(:inv_inner)".
+    wp_load.
+    iDestruct "Hnodes" as "#Hnodes".
+
+    iAssert (
+      [∗ list] node ∈ nodes,
+        ∃ queue,
+        queues_at γ node queue
+    )%I as "#queues_ats".
+    { iApply big_sepL_forall. iIntros "%i %node %Hnodes_lookup".
+      iDestruct (queues_at_get with "Hqueues_auth") as "(%descr & %Hdescrs_lookup & #Hqueues_at)"; first done.
+      iSteps.
+    }
+
+    iSplitR "Hconsumer_queue HΦ". { iFrameSteps. }
+    iIntros "{%} !>".
+
+    awp_smart_apply (bag_2_pop_0_spec with "[- HΦ]"); first iFrameSteps.
+    iApply (aacc_aupd_commit with "HΦ"); first done. iIntros "%vss (:model)". injection Heq as <-.
+    iDestruct (meta_agree with "Hmeta Hmeta_") as %<-. iClear "Hmeta_".
+    iAaccIntro with "Hmodel₁"; first iSteps. iIntros "%o Hmodel₁ !>".
+    iExists o. destruct o as [v |]; last iSteps.
+    iDestruct "Hmodel₁" as "(%producer & %vs & %Hvss_lookup & Hmodel₁)".
+    iSteps.
+  Qed.
   Lemma bag_2_pop_spec t ι consumer :
     <<<
       bag_2_inv t ι ∗
@@ -144,28 +846,68 @@ Section bag_2_G.
     | ∀∀ vss,
       bag_2_model t vss
     >>>
-      bag_2_pop consumer
+      bag_2_pop t consumer @ ↑ι
     <<<
       ∃∃ o,
       match o with
       | None =>
           bag_2_model t vss
       | Some v =>
-          ∃ i v vs,
-          ⌜vss !! i = Some (v :: vs)⌝ ∗
-          bag_2_model t (<[i := vs]> vss)
+          ∃ producer vs,
+          ⌜vss !! producer = Some (v :: vs)⌝ ∗
+          bag_2_model t (<[producer := vs]> vss)
       end
     | RET o;
       bag_2_consumer t consumer
     >>>.
   Proof.
-  Admitted.
-End bag_2_G.
+    iIntros "%Φ ((:inv) & (:consumer)) HΦ". injection Heq as <-.
+    iDestruct (meta_agree with "Hmeta Hmeta_") as %<-. iClear "Hmeta_".
 
-#[global] Opaque bag_2_inv.
-#[global] Opaque bag_2_model.
-#[global] Opaque bag_2_producer.
-#[global] Opaque bag_2_consumer.
+    wp_rec. wp_load.
+    destruct queue as [queue |].
+
+    - iDestruct "Hqueues_elem" as "(:queues_elem)".
+      awp_smart_apply (spmc_queue_pop_spec with "Hqueue_inv") without "Hconsumer_queue".
+      iInv "Hinv" as "(:inv_inner)".
+      iDestruct (queues_at_valid with "Hqueues_auth Hqueues_at") as "(%descr & %Hdescrs_lookup & %Hdescr_queue & %Hwss_lookup)".
+      iDestruct (big_sepM_insert_acc with "Hdescrs") as "((:descriptor_model >) & Hdescrs)"; first done.
+      rewrite -Hdescr_queue.
+      iAaccIntro with "Hqueue_model"; iIntros "Hqueue_model".
+      { iDestruct ("Hdescrs" with "[Hnode_queue Hqueue_model]") as "Hdescrs"; first iSteps.
+        rewrite insert_id //. iFrameSteps.
+      }
+      destruct descr.(descriptor_vals) as [| v vs] eqn:Hdescr_vals => /=.
+
+      + iDestruct ("Hdescrs" with "[Hnode_queue Hqueue_model]") as "Hdescrs".
+        { rewrite -Hdescr_vals. iFrameSteps. }
+        rewrite insert_id //.
+        iSplitR "HΦ". { iFrameSteps. }
+        iIntros "{%} !> _ Hconsumer_queue".
+
+        wp_smart_apply (bag_2_pop_1_spec with "[- HΦ] HΦ").
+        { iSplitR; iSteps. iExists (Some _). iSteps. }
+
+      + iMod "HΦ" as "(%vss & (:model) & _ & HΦ)". injection Heq as <-.
+        iDestruct (meta_agree with "Hmeta Hmeta_") as %<-. iClear "Hmeta_".
+        iDestruct (model_agree with "Hmodel₁ Hmodel₂") as %<-.
+        set vss' :=
+          <[descriptor_to_producer descr node : val := vs]> vss.
+        iMod (model_update vss' with "Hmodel₁ Hmodel₂") as "(Hmodel₁ & Hmodel₂)".
+        iMod ("HΦ" $! (Some v) with "[Hmodel₁]") as "HΦ"; first iSteps.
+
+        iDestruct (queues_update node descr (const vs) with "Hqueues_auth") as "Hqueues_auth"; first done.
+        set descr' :=
+          descriptor_update_vals descr (const vs).
+        iDestruct ("Hdescrs" $! descr' with "[Hnode_queue Hqueue_model]") as "Hdescrs"; first iFrameSteps.
+
+        iSplitR "HΦ". { iFrameSteps. }
+        iSteps. iExists (Some _). iSteps.
+
+    - wp_smart_apply (bag_2_pop_1_spec with "[- HΦ] HΦ").
+      { iSplitR; iSteps. iExists None. iSteps. }
+  Qed.
+End bag_2_G.
 
 #[global] Opaque bag_2_create.
 #[global] Opaque bag_2_create_producer.
@@ -173,3 +915,8 @@ End bag_2_G.
 #[global] Opaque bag_2_create_consumer.
 #[global] Opaque bag_2_push.
 #[global] Opaque bag_2_pop.
+
+#[global] Opaque bag_2_inv.
+#[global] Opaque bag_2_model.
+#[global] Opaque bag_2_producer.
+#[global] Opaque bag_2_consumer.
